Generalized the fairness_preservation over the types of outer trace

fairness/lm_fairness_preservation.v
@@ -18,92 +18,135 @@ Proof.
 Qed.
 
 
-(* Definition lm_exaux_traces_match `{LM:LiveModel (locale Λ) M} `{EqDecision (locale Λ)} : *)
-(*   extrace Λ → auxtrace (LM := LM) → Prop := *)
-(*   traces_match labels_match *)
-(*                live_tids *)
-(*                locale_step *)
-(*                LM.(lm_ls_trans). *)
-
-
 Section fairness_preserved.
-  Context `{LM: LiveModel (locale Λ) M}.
-  Context `{Countable (locale Λ)}.
-  Notation "'Tid'" := (locale Λ).
+  Context `{LM: LiveModel G M}.
+  Context `{EqDecision G}.
 
-  Context (state_rel: cfg Λ → lm_ls LM → Prop).
-  Hypothesis (match_locale_enabled_states: 
+  (* State and labels of 'outer' model.
+     On top level it corresponds to the language. *)
+  (* TODO: formulate it in terms of actual model?
+     Possible for heap_lang but not clear how to do so for arbitrary language
+     (namely, how to uniformly define a state's set of live roles) *)
+  Context {So Lo: Type}.
+  Context `{EqDecision Lo}. 
+
+  Let out_trace := trace So (option Lo).
+
+  (* counterpart of locale step.
+     TODO: any restrictions? *)
+  Context (out_step: So -> option Lo -> So -> Prop). 
+
+  (* Representation of group labels on outer level *)
+  (* TODO: require injectivity? *)
+  Context (lift_grole: G -> Lo).
+  Hypothesis (INJlg: Inj eq eq lift_grole). 
+  
+  (* Context (locale_prop: locale Λ -> cfg Λ -> Prop).  *)
+  Context (locale_prop: Lo -> So -> Prop).
+
+  Definition fair_by (ζ: Lo) (otr: out_trace): Prop :=
+    forall n, pred_at otr n (λ c _, locale_prop ζ c) ->
+         ∃ m, pred_at otr (n+m) (λ c _, ¬ locale_prop ζ c)
+              ∨ pred_at otr (n+m) (λ _ otid, otid = Some (Some ζ)).
+
+
+  (* Context (state_rel: cfg Λ → lm_ls LM → Prop). *)
+  Context (state_rel: So → lm_ls LM → Prop).
+
+  Hypothesis (match_locale_prop_states: 
                forall ζ ρ δ c,
                  ls_mapping δ !! ρ = Some ζ ->
+                 ρ ∈ live_roles _ δ -> 
                  state_rel c δ ->
-                 locale_enabled ζ c). 
+                 (* locale_enabled ζ c *)
+                 locale_prop (lift_grole ζ) c
+             ).
+
+  Definition out_LM_labels_match (oζ : option Lo) (ℓ: lm_lbl LM) :=
+  match oζ with
+  | Some ζ =>
+      exists τ, ζ = lift_grole τ /\
+      match ℓ with
+      | Take_step _ τ' | Silent_step τ' => τ = τ'
+      | Config_step => False
+      end
+  | None => match ℓ with
+           | Config_step => True
+           | _ => False
+           end
+  end. 
 
   (* TODO: rename *)
-  Definition lm_exaux_traces_match_gen: extrace Λ → auxtrace (LM := LM) → Prop :=
+  Definition lm_exaux_traces_match_gen: out_trace → auxtrace (LM := LM) → Prop :=
     traces_match 
-    labels_match
+    (* labels_match *) out_LM_labels_match
     (* live_tids *) state_rel
-    locale_step LM.(lm_ls_trans).
+    (* locale_step  *) out_step
+    LM.(lm_ls_trans).
 
   Lemma traces_match_labels tid ℓ c δ rex (raux : auxtrace (LM := LM)) :
     lm_exaux_traces_match_gen (c -[Some tid]-> rex) (δ -[ℓ]-> raux) ->
-    ((∃ ρ, ℓ = Take_step ρ tid) ∨ (ℓ = Silent_step tid)).
+    exists τ, tid = lift_grole τ /\ 
+    ((∃ ρ, ℓ = Take_step ρ τ) ∨ (ℓ = Silent_step τ)).
   Proof.
     intros Hm. inversion Hm as [|?????? Hlab]; simplify_eq.
+    red in Hlab. destruct Hlab as [? [-> Hlab]]. 
     destruct ℓ; eauto; inversion Hlab; simplify_eq; eauto.
   Qed.
 
-  Lemma mapping_live_role (δ: LiveState Tid M) ρ:
+  Lemma mapping_live_role (δ: LiveState G M) ρ:
     ρ ∈ M.(live_roles) δ ->
-    is_Some (ls_mapping (G := Tid) δ !! ρ).
+    is_Some (ls_mapping δ !! ρ).
   Proof. rewrite -elem_of_dom ls_same_doms. SS. Qed.
-  Lemma fuel_live_role (δ: LiveState Tid M) ρ:
+  Lemma fuel_live_role (δ: LiveState G M) ρ:
     ρ ∈ M.(live_roles) δ ->
-    is_Some (ls_fuel (G := Tid) δ !! ρ).
+    is_Some (ls_fuel δ !! ρ).
   Proof. rewrite -elem_of_dom. SS. Qed.
 
   Local Hint Resolve mapping_live_role: core.
   Local Hint Resolve fuel_live_role: core.
 
-  Lemma match_locale_enabled (extr : extrace Λ) (auxtr : auxtrace (LM := LM)) ζ ρ:
-    lm_exaux_traces_match_gen extr auxtr ->
+  Lemma match_locale_prop (extr : out_trace) (auxtr : auxtrace (LM := LM)) ζ ρ:
+    lm_exaux_traces_match_gen extr auxtr ->    
     ls_mapping (trfirst auxtr) !! ρ = Some ζ ->
-    locale_enabled ζ (trfirst extr).
+    ρ ∈ live_roles _ (trfirst auxtr) ->
+    (* locale_prop ζ (trfirst extr). *)
+    locale_prop (lift_grole ζ) (trfirst extr).
   Proof.
-    intros Hm Hloc.
-    eapply match_locale_enabled_states; eauto.
+    intros Hm Hloc Hlive.
+    eapply match_locale_prop_states; eauto.
     eapply traces_match_first; eauto.  
   Qed. 
   
-  Local Hint Resolve match_locale_enabled: core.
+  (* Local Hint Resolve match_locale_prop: core. *)
   Local Hint Resolve pred_first_trace: core.
 
-  Definition fairness_induction_stmt ρ fm f m ζ extr (auxtr : auxtrace (LM := LM))
+  Definition fairness_induction_stmt ρ fm f m (* ζ *) τ extr (auxtr : auxtrace (LM := LM))
     δ
     (* c *)
     :=
       (infinite_trace extr ->
-       (forall ζ, fair_ex ζ extr) ->
+       (forall ζ, fair_by ζ extr) ->
        fm = (f, m) ->
        lm_exaux_traces_match_gen extr auxtr ->
        (* c = trfirst extr -> *)
        δ = trfirst auxtr ->
        δ.(ls_fuel) !! ρ = Some f ->
-       δ.(ls_mapping) !! ρ = Some ζ ->
-       (pred_at extr m (λ c _, ¬locale_enabled ζ c) ∨ pred_at extr m (λ _ oζ, oζ = Some (Some ζ))) ->
+       δ.(ls_mapping) !! ρ = Some τ ->
+       (pred_at extr m (λ c _, ¬locale_prop (lift_grole τ) c) ∨ pred_at extr m (λ _ oζ, oζ = Some (Some (lift_grole τ)))) ->
       ∃ M, pred_at auxtr M (λ δ _, ¬role_enabled ρ δ)
            ∨ pred_at auxtr M (λ _ ℓ, ∃ ζ0, ℓ = Some (Take_step ρ ζ0))).
 
-  Local Lemma case1 ρ f m (extr' : extrace Λ) (auxtr' : auxtrace (LM := LM)) δ ℓ :
+  Local Lemma case1 ρ f m (extr': out_trace) (auxtr' : auxtrace (LM := LM)) δ ℓ :
     (∀ m0 : nat * nat,
          strict lt_lex m0 (f, m)
-         → ∀ (f m: nat) (ζ: locale Λ) (extr : extrace Λ) (auxtr : auxtrace (LM := LM))
-             (δ : LiveState Tid M) (* (c : cfg Λ) *), fairness_induction_stmt ρ m0 f m ζ extr auxtr δ (* c *)) ->
+         → ∀ (f m: nat) (* (ζ: locale Λ) *) τ (extr : out_trace) (auxtr : auxtrace (LM := LM))
+             (δ : LiveState G M), fairness_induction_stmt ρ m0 f m (* ζ *) τ extr auxtr δ ) ->
     (ρ ∈ dom (ls_fuel (trfirst auxtr')) → oless (ls_fuel (trfirst auxtr') !! ρ) (ls_fuel δ !! ρ)) ->
     lm_exaux_traces_match_gen extr' auxtr' ->
     infinite_trace extr' ->
     ls_fuel δ !! ρ = Some f ->
-    (∀ ζ, fair_ex ζ extr') ->
+    (∀ ζ, fair_by ζ extr') ->
     ∃ M0 : nat,
       pred_at (δ -[ ℓ ]-> auxtr') M0
               (λ δ0 _, ¬ role_enabled ρ δ0)
@@ -117,15 +160,16 @@ Section fairness_preserved.
       destruct (ls_fuel (trfirst auxtr') !! ρ) as [f'|] eqn:Heq.
       - destruct (decide (ρ ∈ live_roles M (trfirst auxtr'))) as [Hρlive'|]; last first.
         { exists 1. left. unfold pred_at. simpl. destruct auxtr'; eauto. }
-        have [ζ' Hζ'] : is_Some (ls_mapping (trfirst auxtr') !! ρ) by eauto.
+        have [τ' Hτ'] : is_Some (ls_mapping (trfirst auxtr') !! ρ) by eauto.
 
-        have Hloc'en: pred_at extr' 0 (λ (c : cfg Λ) (_ : option (olocale Λ)),
-                          locale_enabled ζ' c).
-        { rewrite /pred_at /= pred_first_trace. eauto. }
+        have Hloc'en: pred_at extr' 0 (λ (c : So) (_ : option (option Lo)),
+                          locale_prop (lift_grole τ') c).
+        { rewrite /pred_at /= pred_first_trace.
+          eapply match_locale_prop; eauto. }
 
-        have [p Hp] := (Hfair ζ' 0 Hloc'en).
-        have [P Hind] : ∃ M0 : nat, pred_at auxtr' M0 (λ (δ0 : LiveState Tid M) _, ¬ role_enabled ρ δ0)
-                                  ∨ pred_at auxtr' M0 (λ (_ : LiveState Tid M) ℓ, ∃ ζ0, ℓ = Some (Take_step ρ ζ0)).
+        have [p Hp] := (Hfair (lift_grole τ') 0 Hloc'en).
+        have [P Hind] : ∃ M0 : nat, pred_at auxtr' M0 (λ (δ0 : LiveState G M) _, ¬ role_enabled ρ δ0)
+                                  ∨ pred_at auxtr' M0 (λ (_ : LiveState G M) ℓ, ∃ ζ0, ℓ = Some (Take_step ρ ζ0)).
         { eapply (IH _ _ _ p _ extr'); eauto.
           Unshelve. unfold strict, lt_lex. specialize (Hdec ltac:(by eapply elem_of_dom_2)).
           lia. }
@@ -136,17 +180,18 @@ Section fairness_preserved.
         + apply not_elem_of_dom in Heq; eapply not_elem_of_weaken; last (by apply ls_fuel_dom); set_solver.
     Qed.
 
-    Lemma others_step_fuel_decr ρ f ζ
+    Lemma others_step_fuel_decr ρ f τ
       δ ℓ auxtr' 
       c ζ' extr'
       (Htm: lm_exaux_traces_match_gen (c -[ ζ' ]-> extr') (δ -[ ℓ ]-> auxtr'))
       (Hfuel : ls_fuel δ !! ρ = Some f)
-      (Hmapping : ls_mapping δ !! ρ = Some ζ)
+      (Hmapping : ls_mapping δ !! ρ = Some τ)
       (Hρlive: ρ ∈ live_roles M δ)
-      (Hζ: Some ζ ≠ ζ'):
+      (Hζ: Some (lift_grole τ) ≠ ζ'):
       ∃ f', ls_fuel (trfirst auxtr') !! ρ = Some f' ∧ f' ≤ f.
     Proof.
-      inversion Htm as [|s1 ℓ1 r1 s2 ℓ2 r2 Hl Hs Hts Hls Hmatchrest]; simplify_eq. 
+      inversion Htm as [|s1 ℓ1 r1 s2 ℓ2 r2 Hl Hs Hts Hls Hmatchrest]; simplify_eq.
+      (* red in Hl. *)
       destruct ζ' as [ζ'|]; last first; simpl in *.
       - simpl in *. destruct ℓ; try done. destruct Hls as [_ [_ [Hnoninc _]]].
         have HnotNone: Some ρ ≠ None by congruence.
@@ -155,7 +200,8 @@ Section fairness_preserved.
         destruct (ls_fuel (trfirst auxtr') !! ρ) as [f'|] eqn:Heq; [|set_solver].
         eexists; split =>//. destruct Hnoninc as [Hnoninc|Hnoninc]=>//.
         apply elem_of_dom_2 in Heq. set_solver.
-      - simpl in *. destruct ℓ as [ρ0 ζ0| ζ0|]; try done.
+      - destruct Hl as [τ' [-> Hl]]. 
+        simpl in *. destruct ℓ as [ρ0 ζ0| ζ0|]; try done.
         + destruct Hls as (?&?&?&Hnoninc&?).
           unfold fuel_must_not_incr in Hnoninc.
           have Hneq: Some ρ ≠ Some ρ0 by congruence.
@@ -175,16 +221,16 @@ Section fairness_preserved.
     Qed.
     
     Lemma owner_change_fuel_decr ρ f
-      c ζ extr'
+      c τ extr'
       δ ℓ auxtr'
-      ζ' ζ''
+      ζ' τ''
       (Htm: lm_exaux_traces_match_gen (c -[ ζ' ]-> extr') (δ -[ ℓ ]-> auxtr'))
       (Hfuel: ls_fuel δ !! ρ = Some f)
-      (Hmapping: ls_mapping δ !! ρ = Some ζ)
+      (Hmapping: ls_mapping δ !! ρ = Some τ)
       (Hρlive: ρ ∈ live_roles M δ)
       (Hρlive': ρ ∈ live_roles M (trfirst auxtr'))
-      (Hζ'' : ls_mapping (trfirst auxtr') !! ρ = Some ζ'')
-      (Hchange : ζ ≠ ζ''):
+      (Hζ'' : ls_mapping (trfirst auxtr') !! ρ = Some τ'')
+      (Hchange : τ ≠ τ''):
       ∃ f', ls_fuel (trfirst auxtr') !! ρ = Some f' ∧ f' < f.
     Proof.
       destruct ζ' as [ζ'|]; last first; simpl in *.
@@ -197,7 +243,9 @@ Section fairness_preserved.
         unfold oleq in Hdec. rewrite Hfuel in Hdec.
         destruct (ls_fuel (trfirst auxtr') !! ρ) as [f'|] eqn:Heq; [by eexists|done].
       - inversion Htm as [|s1 ℓ1 r1 s2 ℓ2 r2 Hl Hs Hts Hls Hmatchrest]; simplify_eq.
-        simpl in *. destruct ℓ as [ρ0 ζ0| ζ0|]; try done.
+        simpl in *.
+        destruct Hl as [τ' [-> Hl]]. 
+        destruct ℓ as [ρ0 ζ0| ζ0|]; try done.
         + destruct Hls as (?&?&Hdec&?&?).
           unfold fuel_decr in Hdec. simplify_eq.
           have Hmd: must_decrease ρ (Some ρ0) δ (trfirst auxtr') (Some ζ0).
@@ -214,31 +262,37 @@ Section fairness_preserved.
           destruct (ls_fuel (trfirst auxtr') !! ρ) as [f'|] eqn:Heq; [by eexists|done]. 
     Qed.
 
+    Lemma fair_by_cons :
+∀ (tid : Lo) (c : So) (tid' : option Lo) (r : out_trace),
+  fair_by tid (c -[ tid' ]-> r) → fair_by tid r.
+    Proof. Admitted. 
+
+
 
   Lemma fairness_preserved_ind ρ:
-    ∀ fm f m ζ (extr: extrace Λ) (auxtr: auxtrace (LM := LM)) δ (* c *),
-      fairness_induction_stmt ρ fm f m ζ extr auxtr δ (* c *).
+    ∀ fm f m τ (extr: out_trace) (auxtr: auxtrace (LM := LM)) δ,
+      fairness_induction_stmt ρ fm f m τ extr auxtr δ.
   Proof.
     induction fm as [fm IH] using lex_ind.
-    intros f m ζ extr auxtr δ (* c *) Hexinfin Hfair -> Htm (* -> *) -> Hfuel Hmapping Hexen.
+    intros f m τ extr auxtr δ Hexinfin Hfair -> Htm -> Hfuel Hmapping Hexen.
     destruct extr as [|c ζ' extr'] eqn:Heq.
     { have [??] := Hexinfin 1. done. }
-    have Hfair': (forall ζ, fair_ex ζ extr').
-    { intros. by eapply fair_ex_cons. }
+    have Hfair': (forall τ, fair_by τ extr').
+    { intros. by eapply fair_by_cons. }
     destruct auxtr as [|δ ℓ auxtr']; first by inversion Htm.
     destruct (decide (ρ ∈ live_roles M δ)) as [Hρlive|]; last first.
     { exists 0. left. unfold pred_at. simpl. intros contra. eauto. }
-    destruct (decide (Some ζ = ζ')) as [Hζ|Hζ].
+    destruct (decide (Some (lift_grole τ) = ζ')) as [Hζ|Hζ].
     - rewrite <- Hζ in *.
-
-      (* clear IH.  *)      
-      
-      destruct (traces_match_labels _ _ _ _ _ _ Htm) as [[ρ' ->]| ->]; last first.
+      (* destruct (traces_match_labels _ _ _ _ _ _ Htm) as [[ρ' ->]| ->]; last first. *)
+      destruct (traces_match_labels _ _ _ _ _ _ Htm) as [τ' [LIFT_EQ Htm']].
+      apply INJlg in LIFT_EQ as <-. 
+      destruct Htm' as [[ρ' ->]| ->]; last first.
       + inversion Htm as [|s1 ℓ1 r1 s2 ℓ2 r2 Hl Hs Hts Hls Hmatchrest]; simplify_eq.
         unfold ls_trans in Hls. simpl in Hls. 
         destruct Hls as (? & Hlsdec & Hlsincr).
         unfold fuel_decr in Hlsdec.
-        have Hmustdec: must_decrease ρ None δ (trfirst auxtr') (Some ζ).
+        have Hmustdec: must_decrease ρ None δ (trfirst auxtr') (Some τ).
         { constructor; eauto. }
         eapply case1 =>//.
         * move=> Hinfuel; apply Hlsdec => //; first set_solver.
@@ -253,7 +307,7 @@ Section fairness_preserved.
         { exists 0. right. rewrite /pred_at /=. eauto. }
         destruct Hls as (?&Hsame&Hdec&Hnotinc&_).
         rewrite -Hsame /= in Hmapping.
-        have Hmustdec: must_decrease ρ (Some ρ') δ (trfirst auxtr') (Some ζ).
+        have Hmustdec: must_decrease ρ (Some ρ') δ (trfirst auxtr') (Some τ).
         { constructor; eauto; congruence. }
         (* Copy and paste begins here *)
         eapply case1 =>//; last by eauto using infinite_cons.
@@ -264,16 +318,18 @@ Section fairness_preserved.
       { exists 1. left. unfold pred_at. simpl. destruct auxtr'; eauto. }
       destruct m as [| m'].
       { rewrite -> !pred_at_0 in Hexen. destruct Hexen as [Hexen|Hexen].
-        - exfalso. apply Hexen. unfold locale_enabled. by eapply (match_locale_enabled _ _ _ _ Htm).
+        - exfalso. apply Hexen. eapply (match_locale_prop _ _ _ _ Htm); eauto. 
         - simplify_eq. }
-      have [ζ'' Hζ''] : is_Some (ls_mapping (trfirst auxtr') !! ρ) by eauto.
-      destruct (decide (ζ = ζ'')) as [<-|Hchange].
+      have [τ'' Hτ''] : is_Some (ls_mapping (trfirst auxtr') !! ρ) by eauto.
+      destruct (decide (τ = τ'')) as [<-|Hchange].
       + have [f' [Hfuel' Hff']] : exists f', ls_fuel (trfirst auxtr') !! ρ = Some f' ∧ f' ≤ f.
         { eapply others_step_fuel_decr; eauto. }
 
-        unfold fair_ex in *.
-        have Hζ'en: pred_at extr' 0 (λ (c : cfg Λ) _, locale_enabled ζ c).
-        { rewrite /pred_at /= pred_first_trace. inversion Htm; eauto. }
+        unfold fair_by in *.
+        have Hζ'en: pred_at extr' 0 (λ (c : So) _, locale_prop (lift_grole τ) c).
+        { rewrite /pred_at /= pred_first_trace.
+          eapply match_locale_prop; eauto. 
+          by inversion Htm. }
 
         have [P Hind] : ∃ M0 : nat, pred_at auxtr' M0 (λ δ0 _, ¬ role_enabled ρ δ0)
                         ∨ pred_at auxtr' M0 (λ _ ℓ, ∃ ζ0, ℓ = Some (Take_step ρ ζ0)).
@@ -284,12 +340,16 @@ Section fairness_preserved.
       + have [f' [Hfuel' Hff']] : exists f', ls_fuel (trfirst auxtr') !! ρ = Some f' ∧ f' < f.
         { eapply owner_change_fuel_decr; eauto. }
 
-        unfold fair_ex in *.
-        have: pred_at extr' 0 (λ c _, locale_enabled ζ'' c).
-        { rewrite /pred_at /= pred_first_trace. inversion Htm; eauto. }
-        have Hζ'en: pred_at extr' 0 (λ c _, locale_enabled ζ'' c).
-        { rewrite /pred_at /= pred_first_trace. inversion Htm; eauto. }
-        have [p Hp] := (Hfair' ζ'' 0 Hζ'en).
+        unfold fair_by in *.
+        have: pred_at extr' 0 (λ c _, locale_prop (lift_grole τ'') c).
+        { rewrite /pred_at /= pred_first_trace.
+          eapply match_locale_prop; eauto. 
+          by inversion Htm. }
+        have Hζ'en: pred_at extr' 0 (λ c _, locale_prop (lift_grole τ'') c).
+        { rewrite /pred_at /= pred_first_trace.
+          eapply match_locale_prop; eauto. 
+          by inversion Htm. }
+        have [p Hp] := (Hfair' (lift_grole τ'') 0 Hζ'en).
         have [P Hind] : ∃ M0 : nat, pred_at auxtr' M0 (λ δ0 _, ¬ role_enabled ρ δ0)
                         ∨ pred_at auxtr' M0 (λ _ ℓ, ∃ ζ0, ℓ = Some (Take_step ρ ζ0)).
         { eapply (IH _ _ _ p _ extr'); eauto. by eapply infinite_cons. by inversion Htm.
@@ -297,10 +357,16 @@ Section fairness_preserved.
         exists (1+P). rewrite !pred_at_sum. simpl. done.
   Qed.
 
-  Theorem fairness_preserved (extr: extrace Λ) (auxtr: auxtrace (LM := LM)):
+
+  Lemma fair_by_after :
+    ∀ (ζ : Lo) (tr tr' : out_trace) 
+      (k : nat), after k tr = Some tr' → fair_by ζ tr → fair_by ζ tr'.
+  Proof. Admitted.
+
+  Theorem fairness_preserved (extr: out_trace) (auxtr: auxtrace (LM := LM)):
     infinite_trace extr ->
     lm_exaux_traces_match_gen extr auxtr ->
-    (forall ζ, fair_ex ζ extr) -> (forall ρ, fair_aux ρ auxtr (LM := LM)).
+    (forall ζ, fair_by ζ extr) -> (forall ρ, fair_aux ρ auxtr (LM := LM)).
   Proof.
     intros Hinfin Hmatch Hex ρ n Hn.
 
@@ -312,45 +378,68 @@ Section fairness_preserved.
     setoid_rewrite pred_at_sum. rewrite Heq.
     have Hen: role_enabled ρ (trfirst tr) by destruct tr.
 
-    have [ζ Hζ] : is_Some((trfirst tr).(ls_mapping) !! ρ) by eauto.
+    have [τ Hτ] : is_Some((trfirst tr).(ls_mapping) !! ρ) by eauto.
     have [f Hfuel] : is_Some((trfirst tr).(ls_fuel) !! ρ) by eauto.
-    have Hex' := Hex ζ n.
+    have Hex' := Hex (lift_grole τ) n.
     have [tr1' [Heq' Htr]] : exists tr1', after n extr = Some tr1' ∧ lm_exaux_traces_match_gen tr1' tr
      by eapply traces_match_after.
-    have Hte: locale_enabled ζ (trfirst tr1').
-    { eapply match_locale_enabled; eauto. }
+    have Hte: locale_prop (lift_grole τ) (trfirst tr1').
+    { eapply match_locale_prop.
+      1, 2: eauto.
+      apply Hen. }
     
     setoid_rewrite pred_at_sum in Hex'. rewrite Heq' in Hex'.
-    have Hpa: pred_at extr n (λ c _, locale_enabled ζ c).
+    have Hpa: pred_at extr n (λ c _, locale_prop (lift_grole τ) c).
     { unfold pred_at. rewrite Heq'. destruct tr1'; eauto. }
     destruct (Hex' Hpa) as [m Hm].
     have ?: infinite_trace tr1'.
     { have Hinf := infinite_trace_after n extr Hinfin. by rewrite Heq' in Hinf. }
-    eapply (fairness_preserved_ind ρ _ f m ζ _ tr); eauto.
-    intros ?. by eapply fair_ex_after.
+    eapply (fairness_preserved_ind ρ _ f m τ _ tr); eauto.
+    intros ?. by eapply fair_by_after.
   Qed.
-
-  (* Tactic Notation "inv" open_constr(P) := match goal with *)
-  (*               | [H: P |- _] => inversion H; clear H; simplify_eq *)
-  (*                                         end. *)
 
 End fairness_preserved.
 
-(* TODO: move? *)
-Lemma match_locale_enabled_states_livetids `{EqDecision (locale Λ)}
-  `{LM: LiveModel (locale Λ) M}
-  ζ ρ δ c
-  (Hloc: ls_mapping δ !! ρ = Some ζ)    
-  (Hsr: live_tids c δ (LM := LM)):
-  locale_enabled ζ c. 
-Proof. 
-  rewrite /locale_enabled.
-  destruct Hsr as [HiS Hneqloc]. 
-  have [e Hein] := (HiS _ _ Hloc). exists e. split; first done.
-  destruct (to_val e) eqn:Heqe =>//.
-  exfalso. specialize (Hneqloc ζ e Hein). rewrite Heqe in Hneqloc.
-  have Hv: Some v ≠ None by []. by specialize (Hneqloc Hv ρ).
-Qed. 
 
-Definition lm_exaux_traces_match `{EqDecision (locale Λ)} `{LM: LiveModel (locale Λ) M} :=
-  lm_exaux_traces_match_gen live_tids (LM := LM). 
+(* TODO: move? *)
+Section lang_fairness_preserved.
+  Context `{LM: LiveModel (locale Λ) M}.
+  Context `{Countable (locale Λ)}.
+
+  Definition lm_exaux_traces_match :=
+    lm_exaux_traces_match_gen
+      (locale_step (Λ := Λ))
+      (id: locale Λ -> locale Λ)
+      (live_tids (LM := LM)). 
+
+  Lemma match_locale_enabled_states_livetids
+    ζ ρ δ c
+    (Hloc: ls_mapping δ !! ρ = Some ζ)    
+    (Hsr: live_tids c δ (LM := LM)):
+    locale_enabled ζ c. 
+  Proof. 
+    rewrite /locale_enabled.
+    destruct Hsr as [HiS Hneqloc]. 
+    have [e Hein] := (HiS _ _ Hloc). exists e. split; first done.
+    destruct (to_val e) eqn:Heqe =>//.
+    exfalso. specialize (Hneqloc ζ e Hein). rewrite Heqe in Hneqloc.
+    have Hv: Some v ≠ None by []. by specialize (Hneqloc Hv ρ).
+  Qed. 
+
+  Theorem ex_fairness_preserved (extr: extrace Λ) (auxtr: auxtrace (LM := LM)):
+    infinite_trace extr ->
+    lm_exaux_traces_match extr auxtr ->
+    (forall ζ, fair_ex ζ extr) -> (forall ρ, fair_aux ρ auxtr (LM := LM)).
+  Proof.
+    intros. eapply fairness_preserved; eauto.
+    { apply _. }
+    intros.
+    (* In case of language we don't require the role to be alive,
+       since the notion of thread's "enabledness" is weaker than one of role *)
+    clear H4.
+    eapply match_locale_enabled_states_livetids; eauto.
+    Unshelve. apply _.
+  Qed.
+
+
+End lang_fairness_preserved. 
